\documentclass{article}
\usepackage{ifthen}
\usepackage{epsfig}
\usepackage[utf8]{inputenc}
\usepackage{newunicodechar}
  \newunicodechar{⁻}{${}^{-}$}% Superscript minus
  \newunicodechar{²}{${}^{2}$}% Superscript two
  \newunicodechar{³}{${}^{3}$}% Superscript three

\pagestyle{empty}
\begin{document}
$|a-b|$
\pagebreak

$|a-b|^2$
\pagebreak

$\vec a_i = m_i * \vec g $
\pagebreak

$a-b$
\pagebreak

$ res := res + v*(a+b)$
\pagebreak

$ res := res + v*a$
\pagebreak

$ res := res - a - b$
\pagebreak

$ res := res - v*a$
\pagebreak

$ A $
\pagebreak

$ A = P^TLDL^*P $
\pagebreak

$ a_0, a_1, a_2, ..., a_{n-1}$
\pagebreak

$ a_0 $
\pagebreak

$ a_{i+1}-a_{i}$
\pagebreak

$ a_i $
\pagebreak

$ \ell^p $
\pagebreak

$ \ell^\infty $
\pagebreak

$\infty$
\pagebreak

$ v $
\pagebreak

$ w $
\pagebreak

$ p $
\pagebreak

\[ \Vert v - w \Vert \leqslant p\,\min(\Vert v\Vert, \Vert w\Vert). \]
\pagebreak

$ x $
\pagebreak

\[ \Vert v \Vert \leqslant p\,\vert x\vert. \]
\pagebreak

\[ \Vert v \Vert \leqslant p\,\Vert w\Vert. \]
\pagebreak

$ \{r_0,r_1,..r_{m-1}\} $
\pagebreak

$ \{c_0,c_1,..c_{n-1} \}$
\pagebreak

$ B $
\pagebreak

$ B(i,j) = A(r_i,c_j) $
\pagebreak

$ \sigma $
\pagebreak

$ P_\sigma $
\pagebreak

$ (e_1,\ldots,e_p) $
\pagebreak

\[ P_\sigma(e_i) = e_{\sigma(i)}. \]
\pagebreak

$ \sigma, \tau $
\pagebreak

\[ P_{\sigma\circ\tau} = P_\sigma P_\tau. \]
\pagebreak

$(ij)$
\pagebreak

$ this = this + \alpha u v^* + conj(\alpha) v u^* $
\pagebreak

$ this = this + \alpha ( u u^* ) $
\pagebreak

$ this = this + \alpha ( u^* u ) $
\pagebreak

$ A x = b $
\pagebreak

$ s \Vert \frac{*this}{s} \Vert $
\pagebreak

$[T_{n-1} \ldots T_{i} \ldots T_{0}]$
\pagebreak

$ T_{i} $
\pagebreak

$ T_{i} M$
\pagebreak

$ M T_{i}$
\pagebreak

$ Ax = \lambda B x $
\pagebreak

$ ABx = \lambda x $
\pagebreak

$ BAx = \lambda x $
\pagebreak

$ \lambda $
\pagebreak

$ Av = \lambda v $
\pagebreak

$ D $
\pagebreak

$ V $
\pagebreak

$ A V = V D $
\pagebreak

$ A = V D V^{-1} $
\pagebreak

$ k $
\pagebreak

$ O(n^3) $
\pagebreak

$ n $
\pagebreak

$ A = U T U^*$
\pagebreak

$25n^3$
\pagebreak

$10n^3$
\pagebreak

\[ \begin{bmatrix} u & v \\ -v & u \end{bmatrix} \]
\pagebreak

$ u $
\pagebreak

$ u \pm iv $
\pagebreak

$ AV = VD $
\pagebreak

$ \begin{bmatrix} u & v \\ -v & u \end{bmatrix} $
\pagebreak

$ 25n^3 $
\pagebreak

$ 10n^3 $
\pagebreak

$ Av = \lambda Bv $
\pagebreak

$ A V = B V D $
\pagebreak

$ A = B V D V^{-1} $
\pagebreak

$ \alpha $
\pagebreak

$ \beta $
\pagebreak

$ \lambda_i = \alpha_i / \beta_i $
\pagebreak

$ \beta_i $
\pagebreak

$ \mu = \beta_i / \alpha_i$
\pagebreak

$ \mu_i A v_i = B v_i $
\pagebreak

$ \mu_i u_i^T A = u_i^T B $
\pagebreak

$ u_i $
\pagebreak

$ x^* B x = 1 $
\pagebreak

$ B = LL^* $
\pagebreak

$ L^{-1} A (L^*)^{-1} $
\pagebreak

$ L^{*} A L $
\pagebreak

$ L^{-1} A (L^*)^{-1} (L^* x) = \lambda (L^* x) $
\pagebreak

$ Q $
\pagebreak

$ H $
\pagebreak

$ A = Q H Q^T $
\pagebreak

$ Q^{-1} = Q^T $
\pagebreak

$ A = Q H Q^* $
\pagebreak

$ Q^{-1} = Q^* $
\pagebreak

$ 10n^3/3 $
\pagebreak

$ Q = H_{N-1} \ldots H_1 H_0 $
\pagebreak

$ H_i $
\pagebreak

$ H_i = (I - h_i v_i v_i^T) $
\pagebreak

$ h_i $
\pagebreak

$ i $
\pagebreak

$ v_i $
\pagebreak

$ v_i = [ 0, \ldots, 0, 1, M(i+2,i), \ldots, M(N-1,i) ]^T $
\pagebreak

\[ \|A\|_2 = \max_x \frac{\|Ax\|_2}{\|x\|_2} \]
\pagebreak

$ A^*A $
\pagebreak

$ A = Q S Z $
\pagebreak

$ B = Q T Z $
\pagebreak

$ U^{-1} = U^T $
\pagebreak

$ A - z B $
\pagebreak

$ A = U T U^T $
\pagebreak

$ V^{-1} = V^{\dagger} $
\pagebreak

$ V^{-1} = V^T $
\pagebreak

$ 9n^3 $
\pagebreak

$ 4n^3/3 $
\pagebreak

$ A^{1/2} = V D^{1/2} V^{-1} $
\pagebreak

$ V D^{-1/2} V^{-1} $
\pagebreak

$ A = Q T Q^* $
\pagebreak

$ T $
\pagebreak

$ mat = Q T Q^* $
\pagebreak

$ n \cdot x + d = 0 $
\pagebreak

$ d $
\pagebreak

$ c_0*x_0 + ... + c_{d-1}*x_{d-1} + c_d = 0 $
\pagebreak

$ (\mathbf{a}+i\mathbf{b}) \times (\mathbf{c}+i\mathbf{d}) = (\mathbf{a} \times \mathbf{c} - \mathbf{b} \times \mathbf{d}) - i(\mathbf{a} \times \mathbf{d} - \mathbf{b} \times \mathbf{c})$
\pagebreak

$ \mathbf{o} $
\pagebreak

$ \mathbf{d} $
\pagebreak

$ l(t) = \mathbf{o} + t \mathbf{d} $
\pagebreak

$ t \in \mathbf{R} $
\pagebreak

$ w+xi+yj+zk $
\pagebreak

$ \left( \begin{array}{cc} linear & translation\\ 0 ... 0 & 1 \end{array} \right) $
\pagebreak

$ \left( \begin{array}{cc} I & t \\ 0\,...\,0 & 1 \end{array} \right) $
\pagebreak

$ \left( \begin{array}{cc} R & 0\\ 0\,...\,0 & 1 \end{array} \right) $
\pagebreak

$ \left( \begin{array}{cc} S & 0\\ 0\,...\,0 & 1 \end{array} \right) $
\pagebreak

$ \left( \begin{array}{c} v\\ 1 \end{array} \right) $
\pagebreak

$ \left( \begin{array}{ccc} v_1 & ... & v_n\\ 1 & ... & 1 \end{array} \right) $
\pagebreak

$ c, \mathbf{R}, $
\pagebreak

$ \mathbf{t} $
\pagebreak

\begin{align*} \frac{1}{n} \sum_{i=1}^n \vert\vert y_i - (c\mathbf{R}x_i + \mathbf{t}) \vert\vert_2^2 \end{align*}
\pagebreak

$ \Sigma_{\mathbf{x}\mathbf{y}} \in \mathbb{R}^{d \times d} $
\pagebreak

$ \mathbf{x} $
\pagebreak

$ \mathbf{y} $
\pagebreak

$d$
\pagebreak

$O(d^3)$
\pagebreak

$O(dm)$
\pagebreak

$d \times m$
\pagebreak

$ \mathbf{x} = \left( x_1, \hdots, x_n \right) $
\pagebreak

$ \mathbf{y} = \left( y_1, \hdots, y_n \right) $
\pagebreak

$ c=1 $
\pagebreak

\begin{align*} T = \begin{bmatrix} c\mathbf{R} & \mathbf{t} \\ \mathbf{0} & 1 \end{bmatrix} \end{align*}
\pagebreak

$ H *this = [ beta 0 ... 0]^T $
\pagebreak

$ H = I - tau v v^*$
\pagebreak

$ v^T = [1 essential^T] $
\pagebreak

$ n \times n $
\pagebreak

$ H = \prod_{i=0}^{n-1} H_i $
\pagebreak

$ H_i = I - h_i v_i v_i^* $
\pagebreak

\[ v_i = [\underbrace{0, \ldots, 0}_{i-1\mbox{ zeros}}, 1, \underbrace{*, \ldots,*}_{n-i\mbox{ arbitrary entries}} ]. \]
\pagebreak

$ n-i $
\pagebreak

$ MH $
\pagebreak

$ M $
\pagebreak

$ HM $
\pagebreak

$ H = H_0 H_1 \ldots H_{n-1} $
\pagebreak

$ H = H_{\mathrm{shift}} H_{\mathrm{shift}+1} \ldots H_{n-1} $
\pagebreak

$ S P A P' S \approx L L' $
\pagebreak

$ B = S P A P' S $
\pagebreak

$ \beta > 0 $
\pagebreak

$ B + (\sigma+|\beta| I $
\pagebreak

$ \sigma = 10^{-3} $
\pagebreak

$ \theta $
\pagebreak

$ J = \left ( \begin{array}{cc} c & \overline s \\ -s & \overline c \end{array} \right ) $
\pagebreak

$ v = J^* v $
\pagebreak

$ B = \left ( \begin{array}{cc} x & y \\ \overline y & z \end{array} \right )$
\pagebreak

$ A = J^* B J $
\pagebreak

$ B = \left ( \begin{array}{cc} \text{this}_{pp} & \text{this}_{pq} \\ (\text{this}_{pq})^* & \text{this}_{qq} \end{array} \right )$
\pagebreak

$ G^* $
\pagebreak

$ V = \left ( \begin{array}{c} p \\ q \end{array} \right )$
\pagebreak

$ G^* V = \left ( \begin{array}{c} r \\ 0 \end{array} \right )$
\pagebreak

$ B = \left ( \begin{array}{cc} \text{*this.row}(p) \\ \text{*this.row}(q) \end{array} \right ) $
\pagebreak

$ B = \left ( \begin{array}{cc} \text{*this.col}(p) & \text{*this.col}(q) \end{array} \right ) $
\pagebreak

$ \left ( \begin{array}{cc} x \\ y \end{array} \right ) = J \left ( \begin{array}{cc} x \\ y \end{array} \right ) $
\pagebreak

$ A = P^{-1} L U Q^{-1} $
\pagebreak

$ P^{-1} L U Q^{-1} $
\pagebreak

$ \vert pivot \vert \leqslant threshold \times \vert maxpivot \vert $
\pagebreak

\[ \mathbf{A} \, \mathbf{P} = \mathbf{Q} \, \mathbf{R} \]
\pagebreak

\[ \mathbf{A} \, \mathbf{P} = \mathbf{Q} \, \begin{bmatrix} \mathbf{T} & \mathbf{0} \\ \mathbf{0} & \mathbf{0} \end{bmatrix} \, \mathbf{Z} \]
\pagebreak

$ \mathbf{Z} * \mathbf{rhs} $
\pagebreak

$ \mathbf{\overline Z} * \mathbf{rhs} $
\pagebreak

$ \mathbf{Z}^* * \mathbf{rhs} $
\pagebreak

\[ \mathbf{P} \, \mathbf{A} \, \mathbf{P}' = \mathbf{Q} \, \mathbf{R} \]
\pagebreak

\[ \mathbf{A} = \mathbf{Q} \, \mathbf{R} \]
\pagebreak

$ P_r $
\pagebreak

$P_r A P_c^T = L U$
\pagebreak

$ P_c^T $
\pagebreak

$ A X = B $
\pagebreak

\[ A = U S V^* \]
\pagebreak

$ O(n^2p) $
\pagebreak

$ \vert singular value \vert \leqslant threshold \times \vert max singular value \vert $
\pagebreak

$[-2^{53}+1, 2^{53}-1]$
\pagebreak

\end{document}
